templates/single_copy/link.v
@@ -2,6 +2,7 @@
 
 Require Import lock.
 From iris.algebra Require Import excl auth gmap agree gset frac.
+From iris.algebra.lib Require Import frac_agree.
 From iris.heap_lang Require Export notation locations lang.
 From iris.base_logic.lib Require Export invariants.
 From iris.program_logic Require Export atomic.
@@ -45,18 +46,27 @@ Section Link_Cameras.
 
   (* RA for fractional interfaces *)
   Class fracintG Σ :=
-    FracinthG { fracint_inG :> inG Σ (authR (multiset_flowint_ur K)) }.
-  Definition fracintΣ : gFunctors := #[GFunctor (authR (multiset_flowint_ur K))].
+    FracinthG { fracint_inG :> inG Σ (frac_agreeR (multiset_flowint_ur K)) }.
+  Definition fracintΣ : gFunctors := #[GFunctor (frac_agreeR (multiset_flowint_ur K))].
 
   Instance subG_fracintΣ {Σ} : subG fracintΣ Σ → fracintG Σ.
   Proof. solve_inG. Qed.
+
+  (* RA for ghost locations *)
+  Class ghost_heapG Σ :=
+    Ghost_heapG { ghost_heap_inG :> inG Σ (authR $ gmapUR Node $ agreeR $ prodO gnameO gnameO) }.
+  Definition ghost_heapΣ : gFunctors := #[GFunctor (authR $ gmapUR Node $ agreeR $ prodO gnameO gnameO)].
+
+  Instance subG_ghost_heapΣ {Σ} : subG ghost_heapΣ Σ → ghost_heapG Σ.
+  Proof. solve_inG. Qed.
+
 
 End Link_Cameras.
 
 (** Verification of the template *)
 Section Link_Template.
   Context `{!heapG Σ, !flowintG Σ, !nodesetG Σ, !(@keysetG K _ _) Σ, !inreachG Σ,
-    !fracintG Σ}.
+    !fracintG Σ, !ghost_heapG Σ}.
   Notation iProp := (iProp Σ).
 
   (** The code of the link template. *)
@@ -67,8 +77,14 @@ Section Link_Template.
 
   (* TODO add alias inreach = inset for this file. *)
 
+  Parameter createRoot : val.
   Parameter findNext : val.
   Parameter decisiveOp : (dOp → val).
+
+  Definition init : val :=
+    λ: <>,
+      let: "r" := createRoot #() in
+      "r".
 
   Definition traverse : val :=
     rec: "tr" "n" "k" :=
@@ -109,6 +125,15 @@ Section Link_Template.
   (* The following specs are proved for each implementation in GRASShopper
    * (see b-link.spl and hashtbl-link.spl *)
 
+  Parameter createRoot_spec :
+      ⊢ ({{{ True }}}
+           createRoot #()
+         {{{ (r: Node) (Ir: multiset_flowint_ur K) (ks: nzmap K nat),
+             RET #r; node r Ir ∅ ∗ (lockLoc r) ↦ #false 
+                     ∗ ⌜Ir = int {| infR := {[r := ks]}; outR := ∅ |}⌝
+                     ∗ ⌜dom (gset K) ks = KS⌝
+                     }}})%I.
+
   Parameter findNext_spec : ∀ (n: Node) (k: K) (In : multiset_flowint_ur K) (C: gset K),
     ⊢ ({{{ ⌜k ∈ KS⌝ ∗ node n In C ∗ ⌜in_inset K k In n⌝ }}}
          findNext #n #k
@@ -133,46 +158,49 @@ Section Link_Template.
   Definition inFP γ_f n : iProp :=
     ∃ (N: gset Node), own γ_f (◯ N) ∗ ⌜n ∈ N⌝.
 
-  Definition inInr γ_i k (n: Node) : iProp :=
-    ∃ (Ks: gset K), own (γ_i n) (◯ Ks) ∗ ⌜k ∈ Ks⌝.
+  Definition inInr γ_in k : iProp :=
+    ∃ (Ks: gset K), own (γ_in) (◯ Ks) ∗ ⌜k ∈ Ks⌝.
 
-  Definition nodePred γ_f γ_h γ_k n In Cn : iProp :=
-    node n In Cn
-    ∗ own (γ_h n) ((●{1/2} In))
+  Definition nodePred γ_f γ_gh γ_k n In Cn : iProp :=
+    ∃ γ_hn γ_in, 
+      node n In Cn
+    ∗ own (γ_hn) ((to_frac_agree (1/2) In))
     ∗ own γ_k (◯ prod (keyset K In n, Cn))
     ∗ inFP γ_f n
-    ∗ ⌜domm In = {[n]}⌝.
+    ∗ own γ_gh (◯ {[n := to_agree (γ_hn, γ_in)]}).
 
-  Definition nodeShared γ_I γ_i γ_h n In : iProp :=
-    own γ_I (◯ In)
-    ∗ own (γ_h n) ((●{1/2} In))
+  Definition nodeShared γ_I γ_gh n In : iProp :=
+    ∃ γ_hn γ_in,  
+      own γ_I (◯ In)
+    ∗ own (γ_hn) ((to_frac_agree (1/2) In))
     ∗ ⌜domm In = {[n]}⌝    (* Needed for globalinv_root_ins *)
-    ∗ own (γ_i n) (● (inset K In n)).
+    ∗ own (γ_in) (● (inset K In n))
+    ∗ own γ_gh (◯ {[n := to_agree (γ_hn, γ_in)]}).
 
-  Definition nodeFull γ_I γ_f γ_k γ_i γ_h n : iProp :=
+  Definition nodeFull γ_I γ_f γ_k γ_gh n : iProp :=
     (∃ (b: bool) In Cn,
-        lockR b n (nodePred γ_f γ_h γ_k n In Cn)
-        ∗ nodeShared γ_I γ_i γ_h n In).
+        lockR b n (nodePred γ_f γ_gh γ_k n In Cn)
+        ∗ nodeShared γ_I γ_gh n In).
   
-  Definition globalGhost γ_I γ_k γ_f r I C : iProp :=
+  Definition globalGhost γ_I γ_k γ_f γ_gh hγ r I C : iProp :=
     (own γ_I (● I) ∗ ⌜globalinv K r I⌝ ∗ own γ_k (● prod (KS, C))
-     ∗ own γ_f (● domm I))%I.
+     ∗ own γ_f (● domm I) ∗ own γ_gh (● hγ)).
 
-  Definition CSSi γ_I γ_f γ_k γ_i γ_h r C I : iProp :=
-    (globalGhost γ_I γ_k γ_f r I C
-     ∗ ([∗ set] n ∈ (domm I), nodeFull γ_I γ_f γ_k γ_i γ_h n)
+  Definition CSSi γ_I γ_f γ_k γ_gh hγ r C I : iProp :=
+    (globalGhost γ_I γ_k γ_f γ_gh hγ r I C
+     ∗ ([∗ set] n ∈ (domm I), nodeFull γ_I γ_f γ_k γ_gh n)
     )%I.
 
-  Definition CSS γ_I γ_f γ_k γ_i γ_h r C : iProp :=
-    (∃ I, CSSi γ_I γ_f γ_k γ_i γ_h r C I)%I.
+  Definition CSS γ_I γ_f γ_k γ_gh r C : iProp :=
+    (∃ hγ I, CSSi γ_I γ_f γ_k γ_gh hγ r C I)%I.
 
   (** Some useful lemmas *)
 
-  Lemma inFP_domm γ_I γ_f γ_k γ_i γ_h r C I n :
-    inFP γ_f n -∗ CSSi γ_I γ_f γ_k γ_i γ_h r C I -∗ ⌜n ∈ domm I⌝.
+  Lemma inFP_domm γ_I γ_f γ_k γ_gh hγ r C I n :
+    inFP γ_f n -∗ CSSi γ_I γ_f γ_k γ_gh hγ r C I -∗ ⌜n ∈ domm I⌝.
   Proof.
     iIntros "#Hfp Hcss".
-    iDestruct "Hcss" as "((HI & Hglob & Hks & Hdom) & Hbigstar)".
+    iDestruct "Hcss" as "((HI & Hglob & Hks & Hdom & Hgh) & Hbigstar)".
     iDestruct "Hfp" as (N) "(#Hdom' & n_in_N)". iDestruct "n_in_N" as %n_in_N.
     iPoseProof ((auth_own_incl γ_f (domm I) N) with "[$]") as "#N_incl".
     iDestruct "N_incl" as %N_incl.
@@ -180,104 +208,137 @@ Section Link_Template.
     iPureIntro. set_solver.
   Qed.
   
-  Lemma frac_int_equal (γ_h: Node → gname) n In In' :
-    own (γ_h n) (●{1/2} In) -∗ own (γ_h n) (●{1/2} In') -∗ ⌜In = In'⌝.
+  Lemma frac_int_equal γ_hn In In' :
+    own γ_hn (to_frac_agree (1/2) In) -∗ own γ_hn (to_frac_agree (1/2) In') -∗ ⌜In = In'⌝.
   Proof.
     iIntros.
-    iPoseProof ((own_valid_2 (γ_h n) (●{1/2} In) (●{1/2} In'))
+    iPoseProof ((own_valid_2 (γ_hn) (to_frac_agree (1/2) In) (to_frac_agree (1/2) In'))
                   with "[$] [$]") as "%"; try done.
     iPureIntro.
-    apply (auth_auth_frac_op_inv _ _ _ _) in H0.
+    apply frac_agree_op_valid in H0.
+    destruct H0 as [_ H0].
     by apply leibniz_equiv.
   Qed.
     
-  Lemma CSS_unfold γ_I γ_f γ_k γ_i γ_h r C n :
-    CSS γ_I γ_f γ_k γ_i γ_h r C -∗ inFP γ_f n
-    -∗ (∃ I, globalGhost γ_I γ_k γ_f r I C ∗ nodeFull γ_I γ_f γ_k γ_i γ_h n
+  Lemma CSS_unfold γ_I γ_f γ_k γ_gh r C n :
+    CSS γ_I γ_f γ_k γ_gh r C -∗ inFP γ_f n
+    -∗ (∃ hγ I, globalGhost γ_I γ_k γ_f γ_gh hγ r I C 
+        ∗ nodeFull γ_I γ_f γ_k γ_gh n
         ∗ (∀ C',
-           globalGhost γ_I γ_k γ_f r I C' ∗ nodeFull γ_I γ_f γ_k γ_i γ_h n
-           -∗ CSS γ_I γ_f γ_k γ_i γ_h r C')).
+           globalGhost γ_I γ_k γ_f γ_gh hγ r I C' ∗ nodeFull γ_I γ_f γ_k γ_gh n
+           -∗ CSS γ_I γ_f γ_k γ_gh r C')).
   Proof.
     iIntros "Hcss #Hfp".
-    iDestruct "Hcss" as (I) "((HI & Hglob & Hks & Hdom) & Hbigstar)".
+    iDestruct "Hcss" as (hγ I) "((HI & Hglob & Hks & Hdom & Hgh) & Hbigstar)".
     iPoseProof (inFP_domm with "[$] [$]") as "%".
     rewrite (big_sepS_elem_of_acc _ (domm I) n); last by eauto.
-    iDestruct "Hbigstar" as "(Hn & Hbigstar)". iExists I. iFrame "∗".
+    iDestruct "Hbigstar" as "(Hn & Hbigstar)". iExists hγ, I. iFrame "∗".
     iIntros (C') "((HI & Hglob & Hks & Hdom) & H)".
-    iExists I. iFrame "∗". by iApply "Hbigstar".
+    iExists hγ, I. iFrame "∗". by iApply "Hbigstar".
   Qed.
 
-  Lemma node_nodeFull_equal γ_I γ_f γ_k γ_i γ_h n In Cn :
-    node n In Cn -∗ own (γ_h n) (●{1/2} In) -∗ nodeFull γ_I γ_f γ_k γ_i γ_h n
-    -∗ ((lockR true n (∃ In Cn, nodePred γ_f γ_h γ_k n In Cn)) ∗ node n In Cn ∗ own (γ_h n) (●{1/2} In)
-        ∗ nodeShared γ_I γ_i γ_h n In).
+  Lemma ghost_heap_sync γ_gh n γ_hn γ_hn' γ_in γ_in' :
+    own γ_gh (◯ {[n := to_agree (γ_hn, γ_in)]})
+      -∗ own γ_gh (◯ {[n := to_agree (γ_hn', γ_in')]})
+          -∗ ⌜γ_hn = γ_hn'⌝ ∗ ⌜γ_in = γ_in'⌝.
   Proof.
-    iIntros "Hn HhIn Hnf".
+    iIntros "H1 H2". iCombine "H1" "H2" as "H".
+    iPoseProof (own_valid with "H") as "Valid".
+    iDestruct "Valid" as %Valid.
+    rewrite auth_frag_valid in Valid *; intros Valid.
+    apply singleton_valid in Valid.
+    apply to_agree_op_inv in Valid.
+    apply leibniz_equiv in Valid.
+    inversion Valid.
+    by iPureIntro.
+  Qed.
+
+  Lemma node_nodeFull_equal γ_I γ_f γ_k γ_gh γ_hn γ_in n In Cn :
+    node n In Cn -∗ 
+      own γ_gh (◯ {[n := to_agree (γ_hn, γ_in)]}) -∗ 
+        own (γ_hn) (to_frac_agree (1/2) In) -∗ 
+          nodeFull γ_I γ_f γ_k γ_gh n -∗ 
+            ((lockR true n (∃ In Cn, nodePred γ_f γ_gh γ_k n In Cn)) 
+              ∗ node n In Cn ∗ own (γ_hn) (to_frac_agree (1/2) In)
+              ∗ nodeShared γ_I γ_gh n In).
+  Proof.
+    iIntros "Hn #Hgh HhIn Hnf".
     iDestruct "Hnf" as (b In' Cn') "(Hlock & Hns)". 
     destruct b.
     - (* Case n locked *)
       iFrame "Hlock".
-      iDestruct "Hns" as "(Hns & Hnp)".
-      iDestruct "Hnp" as "(HhIn' & HdomIn)".
+      iDestruct "Hns" as (γ_hn' γ_in')"(Hns & HhIn' & HdomIn & Hinr & #Hgh')".
+      iPoseProof (ghost_heap_sync _ _ _ _ with "[$Hgh] [$Hgh']") as "(% & %)". subst γ_hn' γ_in'.
       iPoseProof (frac_int_equal with "[$] [$]") as "%". subst In'.
-      iFrame "∗".
+      iFrame "∗". iExists γ_hn, γ_in. iFrame "∗#".
     - (* Case n unlocked: impossible *)
       iDestruct "Hlock" as "(H & Hnp)".
-      iDestruct "Hnp" as "(Hn' & _)".
+      iDestruct "Hnp" as (? ?)"(Hn' & _)".
       iExFalso. iApply (node_sep_star n In In' with "[$]").
   Qed.
 
-  Lemma CSS_unfold_node_wand γ_I γ_f γ_k γ_i γ_h r C n In Cn :
-    CSS γ_I γ_f γ_k γ_i γ_h r C
-    -∗ node n In Cn -∗ own (γ_h n) (●{1/2} In) -∗ inFP γ_f n
-    -∗ (∃ I, node n In Cn ∗ own (γ_h n) (●{1/2} In)
-        ∗ globalGhost γ_I γ_k γ_f r I C
-        ∗ (lockR true n (nodePred γ_f γ_h γ_k n In Cn)) ∗ nodeShared γ_I γ_i γ_h n In
-        ∗ (∀ C',
-          globalGhost γ_I γ_k γ_f r I C' ∗ nodeFull γ_I γ_f γ_k γ_i γ_h n
-          -∗ CSS γ_I γ_f γ_k γ_i γ_h r C')).
+  Lemma CSS_unfold_node_wand γ_I γ_f γ_k γ_gh γ_hn γ_in r C n In Cn :
+    CSS γ_I γ_f γ_k γ_gh r C -∗ 
+      node n In Cn -∗ own γ_gh (◯ {[n := to_agree (γ_hn, γ_in)]}) -∗
+        own (γ_hn) (to_frac_agree (1/2) In) -∗ 
+          inFP γ_f n -∗ 
+            (∃ hγ I, node n In Cn 
+                  ∗ own (γ_hn) (to_frac_agree (1/2) In)
+                  ∗ globalGhost γ_I γ_k γ_f γ_gh hγ r I C
+                  ∗ (lockR true n (nodePred γ_f γ_gh γ_k n In Cn)) 
+                  ∗ nodeShared γ_I γ_gh n In
+                  ∗ (∀ C', globalGhost γ_I γ_k γ_f γ_gh hγ r I C' 
+                            ∗ nodeFull γ_I γ_f γ_k γ_gh n -∗ 
+                                CSS γ_I γ_f γ_k γ_gh r C')).
   Proof.
-    iIntros "Hcss Hn HhIn #Hfp".
-    iPoseProof (CSS_unfold with "[$] [$]") as (I) "(Hg & Hnf & Hcss')".
-    iExists I.
-    iPoseProof (node_nodeFull_equal with "[$] [$] [$]")
+    iIntros "Hcss Hn #Hgh HhIn #Hfp".
+    iPoseProof (CSS_unfold with "[$] [$]") as (hγ I) "(Hg & Hnf & Hcss')".
+    iExists hγ, I.
+    iPoseProof (node_nodeFull_equal with "[$] [$] [$] [$]")
       as "(Hlock & H' & Hn & Hn')". 
-      iDestruct "Hlock" as "(Hlock' & H)".
+    iDestruct "Hlock" as "(Hlock' & H)".
     iFrame.
   Qed.
 
-  Lemma CSS_unfold_node γ_I γ_f γ_k γ_i γ_h r C n In Cn :
-    CSS γ_I γ_f γ_k γ_i γ_h r C
-    -∗ node n In Cn -∗ own (γ_h n) (●{1/2} In) -∗ inFP γ_f n
-    -∗ (∃ I, node n In Cn ∗ own (γ_h n) (●{1/2} In)
-        ∗ globalGhost γ_I γ_k γ_f r I C
-        ∗ lockR true n (∃ In Cn, nodePred γ_f γ_h γ_k n In Cn)
-        ∗ nodeShared γ_I γ_i γ_h n In
-        ∗ ([∗ set] n' ∈ (domm I ∖ {[n]}), nodeFull γ_I γ_f γ_k γ_i γ_h n')).
+  Lemma CSS_unfold_node γ_I γ_f γ_k γ_gh γ_hn γ_in r C n In Cn :
+    CSS γ_I γ_f γ_k γ_gh r C -∗ 
+      node n In Cn -∗ own γ_gh (◯ {[n := to_agree (γ_hn, γ_in)]}) -∗
+        own (γ_hn) (to_frac_agree (1/2) In) -∗ 
+          inFP γ_f n -∗ 
+            (∃ hγ I, node n In Cn ∗ own (γ_hn) (to_frac_agree (1/2) In)
+                  ∗ globalGhost γ_I γ_k γ_f γ_gh hγ r I C
+                  ∗ lockR true n (∃ In Cn, nodePred γ_f γ_gh γ_k n In Cn)
+                  ∗ nodeShared γ_I γ_gh n In
+                  ∗ ([∗ set] n' ∈ (domm I ∖ {[n]}), nodeFull γ_I γ_f γ_k γ_gh n')).
   Proof.
-    iIntros "Hcss Hn HhIn #Hfp".
-    iDestruct "Hcss" as (I) "(Hgl & Hbigstar)".
+    iIntros "Hcss Hn #Hgh HhIn #Hfp".
+    iDestruct "Hcss" as (hγ I) "(Hgl & Hbigstar)".
     iPoseProof (inFP_domm with "[$] [$]") as "%".
     rewrite (big_sepS_delete _ (domm I) n); last by eauto.
     iDestruct "Hbigstar" as "(Hnf & Hbigstar)".
-    iPoseProof (node_nodeFull_equal with "[$] [$] [$]")
+    iPoseProof (node_nodeFull_equal with "[$] [$] [$] [$]")
       as "(Hlock & Hn & HhIn &Hns)".
-    iExists I. iFrame.
+    iExists hγ, I. iFrame.
   Qed.
 
-  Lemma inInr_impl_inset γ_I γ_f γ_k γ_i γ_h r C n In Cn k :
-    CSS γ_I γ_f γ_k γ_i γ_h r C -∗ nodePred γ_f γ_h γ_k n In Cn
-    -∗ inInr γ_i k n
-    -∗ ⌜in_inset K k In n⌝.
+  Lemma inInr_impl_inset γ_I γ_f γ_k γ_gh γ_hn γ_in r C n In Cn k :
+    CSS γ_I γ_f γ_k γ_gh r C -∗ 
+      nodePred γ_f γ_gh γ_k n In Cn -∗
+        own γ_gh (◯ {[n := to_agree (γ_hn, γ_in)]}) -∗ 
+          inInr γ_in k -∗ ⌜in_inset K k In n⌝.
   Proof.
-    iIntros "Hcss Hnp Hinr".
-    iDestruct "Hnp" as "(Hn & HnhIn & HkIn & #Hinfp & domIn)".
-    iPoseProof (CSS_unfold_node with "[$] [$] [$] [$]")
-      as (I) "(Hn & HhIn & Hg & Hlock & Hns & Hcss')".
-    iDestruct "Hg" as "(HI & Hglob & Hks & Hdom)".
-    iDestruct "Hns" as "(HIn & HhIn' & HdomIn & Hins)".
+    iIntros "Hcss Hnp #Hgh' Hinr".
+    iDestruct "Hnp" as (γ_hn' γ_in')"(Hn & HnhIn & HkIn & #Hinfp & #Hgh)".
+    iPoseProof (ghost_heap_sync _ _ _ _ with "[$Hgh] [$Hgh']") as "(% & %)". 
+    subst γ_hn' γ_in'.
+    iPoseProof (CSS_unfold_node with "[$] [$] [$] [$] [$]")
+      as (hγ I) "(Hn & HhIn & Hg & Hlock & Hns & Hcss')".
+    iDestruct "Hg" as "(HI & Hglob & Hks & Hdom & Hγ)".
+    iDestruct "Hns" as (γ_hn' γ_in')"(HIn & HhIn' & HdomIn & Hins & #Hgh'')".
     iDestruct "Hinr" as (R) "(Hinr & %)".
-    iPoseProof ((auth_own_incl (γ_i n) (inset K In n) R) with "[$]")
+    iPoseProof (ghost_heap_sync _ _ _ _ with "[$Hgh] [$Hgh'']") as "(% & %)". 
+    subst γ_hn' γ_in'.
+    iPoseProof ((auth_own_incl (γ_in) (inset K In n) R) with "[$]")
       as "incl".
     iDestruct "incl" as %incl. iPureIntro.
     apply gset_included in incl. set_solver.
@@ -295,30 +356,33 @@ Section Link_Template.
   Qed.
 
   (* Can we unify this with the above? *)
-  Lemma ghost_snapshot_fp_k γ_i (Ks: gset K) k n :
-    ⊢ own (γ_i n) (● Ks) -∗ ⌜k ∈ Ks⌝ ==∗ own (γ_i n) (● Ks) ∗ inInr γ_i k n.
+  Lemma ghost_snapshot_fp_k γ_in (Ks: gset K) k :
+    ⊢ own (γ_in) (● Ks) -∗ ⌜k ∈ Ks⌝ ==∗ own (γ_in) (● Ks) ∗ inInr γ_in k.
   Proof.
     iIntros.
-    iMod (own_update (γ_i n) (● Ks) (● Ks ⋅ ◯ Ks) with "[$]")
+    iMod (own_update (γ_in) (● Ks) (● Ks ⋅ ◯ Ks) with "[$]")
       as "H".
     { apply auth_update_frac_alloc. apply gset_core_id. done. }
     iDestruct "H" as "(Haa & Haf)". iFrame. iModIntro.
     iExists Ks. by iFrame.
   Qed.
     
-  Lemma ghost_update_step γ_I γ_f γ_k γ_i γ_h r C n In Cn k n' :
-    ⊢ CSS γ_I γ_f γ_k γ_i γ_h r C
-      -∗ nodePred γ_f γ_h γ_k n In Cn
+  Lemma ghost_update_step γ_I γ_f γ_k γ_gh r C n In Cn k n' :
+    ⊢ CSS γ_I γ_f γ_k γ_gh r C
+      -∗ nodePred γ_f γ_gh γ_k n In Cn
       -∗ ⌜in_inset K k In n⌝
       -∗ ⌜in_outset K k In n'⌝
-      ==∗ CSS γ_I γ_f γ_k γ_i γ_h r C ∗ nodePred γ_f γ_h γ_k n In Cn
-      ∗ inFP γ_f n' ∗ inInr γ_i k n'.
+      ==∗ ∃ γ_hn' γ_in', CSS γ_I γ_f γ_k γ_gh r C ∗ nodePred γ_f γ_gh γ_k n In Cn
+      ∗ own γ_gh (◯ {[n' := to_agree (γ_hn', γ_in')]}) 
+      ∗ inFP γ_f n' ∗ inInr γ_in' k.
   Proof.
     iIntros "Hcss Hnp % %".
-    iDestruct "Hnp" as "(Hn & HnhIn & HkIn & #Hinfp & %)".
-    iPoseProof (CSS_unfold_node with "[$] [$] [$] [$]")
-      as (I) "(Hn & HhIn & (HI & % & Hks & Hdom) & Hlock & Hns & Hbigstar)".
-    iDestruct "Hns" as "(HIn & HhInn & % & Hins)".
+    iDestruct "Hnp" as (γ_hn γ_in)"(Hn & HnhIn & HkIn & #Hinfp & #Hgh)".
+    iPoseProof (CSS_unfold_node with "[$] [$] [$] [$] [$]")
+      as (hγ I) "(Hn & HhIn & (HI & % & Hks & Hdom & Hγ) & Hlock & Hns & Hbigstar)".
+    iDestruct "Hns" as (γ_hn' γ_in')"(HIn & HhInn & % & Hins & #Hgh')".
+    iPoseProof (ghost_heap_sync _ _ _ _ with "[$Hgh] [$Hgh']") as "(% & %)". 
+    subst γ_hn' γ_in'.    
     (* In ≼ I *)
     iPoseProof ((auth_own_incl γ_I I In) with "[$]")
       as (Io) "#incl".
@@ -329,8 +393,9 @@ Section Link_Template.
     (* Prove the preconditions of ghost_snapshot_fp *)
     assert (n' ∈ domm Io). 
     { apply (flowint_step I In Io k); try done.
-        by rewrite auth_auth_valid in H5 *.
-        unfold globalinv in H3. destruct H3 as (_ & _ & cI & _). done.
+      by apply auth_auth_valid.
+      unfold globalinv in H2. destruct H2 as (_ & _ & cI & _).
+      done.
     }
     assert (domm I = domm In ∪ domm Io). {
       rewrite incl. rewrite flowint_comp_fp. done.
@@ -354,7 +419,8 @@ Section Link_Template.
     iDestruct "Hbigstar" as "(Hnf' & Hbigstar)".
     (* Get ✓ (In ⋅ In') *)
     iDestruct "Hnf'" as (b In' Cn') "(? & HInn)".
-    iDestruct "HInn" as "(HInn & (HIn' & % & Hins'))".
+    iClear "Hgh'".
+    iDestruct "HInn" as (γ_hn' γ_in') "(HInn & (HIn' & % & Hins' & #Hgh'))".
     iAssert (✓ (In ⋅ In'))%I as "%". {
       iPoseProof ((own_op γ_I (◯ In) (◯ In' )) with "[HIn HInn]") as "H";
         first by eauto with iFrame.
@@ -367,34 +433,37 @@ Section Link_Template.
       set_solver. set_solver.
     }
     (* snapshot In' inreach to get inInr k n' *)
-    iMod (ghost_snapshot_fp_k γ_i _ k n' with "[$] [% //]")
+    iMod (ghost_snapshot_fp_k γ_in' _ k with "[$] [% //]")
       as "(Hins' & #Hininr')".
     (* Aaaand, we're done *)
     iModIntro.
-    iAssert (CSS γ_I γ_f γ_k γ_i γ_h r C)%I with "[-Hn HkIn HhInn]" as "Hcss". 
+    iAssert (CSS γ_I γ_f γ_k γ_gh r C)%I with "[-Hn HkIn HhInn]" as "Hcss". 
     {
-      iExists I. iFrame "HI Hks Hdom".
+      iExists hγ, I. iFrame "HI Hks Hdom Hγ".
       iSplitR. by iPureIntro.
       rewrite (big_sepS_delete _ (domm I) n); last by eauto.
       iSplitL "Hlock HIn HhIn Hins".
       iExists true, In, Cn. iSplitR "HIn HhIn Hins". eauto with iFrame. 
-      iFrame "%". iFrame "∗".
+      iExists γ_hn, γ_in. iFrame "∗%#".
       rewrite (big_sepS_delete _ (domm I ∖ {[n]}) n'); last by eauto.
       iFrame "Hbigstar".
       iExists b, In', Cn'. iSplitR "HIn' Hins' HInn". eauto with iFrame.
-      iFrame "%". iFrame "∗". 
+      iFrame "%". iExists γ_hn', γ_in'. iFrame "∗#". 
     }
-    iFrame "#". iFrame "∗". by iPureIntro.
+    iExists γ_hn', γ_in'. iFrame "#". iFrame "∗". iExists γ_hn, γ_in. 
+    iFrame "#∗".
   Qed.
 
-  Lemma ghost_update_root γ_I γ_f γ_k γ_i γ_h r C k :
-    ⊢ CSS γ_I γ_f γ_k γ_i γ_h r C -∗ ⌜k ∈ KS⌝
+  Lemma ghost_update_root γ_I γ_f γ_k γ_gh r C k :
+    ⊢ CSS γ_I γ_f γ_k γ_gh r C -∗ ⌜k ∈ KS⌝
       ==∗
-      CSS γ_I γ_f γ_k γ_i γ_h r C ∗ inFP γ_f r ∗ inInr γ_i k r.
+      ∃ γ_hr γ_ir, CSS γ_I γ_f γ_k γ_gh r C
+        ∗ own γ_gh (◯ {[r := to_agree (γ_hr, γ_ir)]}) 
+        ∗ inFP γ_f r ∗ inInr γ_ir k.
   Proof.
     iIntros "Hcss %".
     (* Open CSS to get r ∈ domm I *)
-    iDestruct "Hcss" as (I) "((HI & #Hglob & Hks & Hdom) & Hbigstar)".
+    iDestruct "Hcss" as (hγ I) "((HI & #Hglob & Hks & Hdom & Hγ) & Hbigstar)".
     iDestruct "Hglob" as %Hglob.
     assert (r ∈ domm I)%I as Hroot.
     { apply globalinv_root_fp. done. }
@@ -405,30 +474,32 @@ Section Link_Template.
     rewrite (big_sepS_elem_of_acc _ (domm I) r); last by eauto.
     iDestruct "Hbigstar" as "(Hnf & Hbigstar)".
     iDestruct "Hnf" as (b Ir Cr) "(Hlock & Hnp)".
-    iDestruct "Hnp" as "(HIn & HhInn & % & Hins)".
+    iDestruct "Hnp" as (γ_hr γ_ir)"(HIn & HhInn & % & Hins & #Hgh)".
     (* Get Ir ≼ I needed for globalinv_root_ins *)
-    iPoseProof (auth_own_incl with "[$HI $HIn]") as "%".
-    iMod (own_update (γ_i r) _ (● (inset K Ir r) ⋅ ◯ (inset K Ir r))
+    iPoseProof (auth_own_incl _ I Ir with "[$HI $HIn]") as "%".
+    iMod (own_update (γ_ir) _ (● (inset K Ir r) ⋅ ◯ (inset K Ir r))
             with "Hins") as "(Hins & #Hinr)".
     { apply auth_update_frac_alloc. apply gset_core_id. done. }
     (* Hksr -> Hinr *)
-    iAssert (inInr γ_i k r)%I as "#Hininr".
+    iAssert (inInr γ_ir k)%I as "#Hininr".
     {
       iExists (inset K Ir r). iFrame "Hinr". iPureIntro.
       apply (globalinv_root_ins I). done. 
     }
-    iModIntro. iSplitL. iExists I. iFrame "∗". iSplitR; first by iPureIntro.
-    iApply "Hbigstar". iExists b, Ir, Cr. iFrame "∗". iFrame "%". iFrame "#".
+    iModIntro. iExists γ_hr, γ_ir. iSplitL. 
+    iExists hγ, I. iFrame "∗". iSplitR; first by iPureIntro.
+    iApply "Hbigstar". iExists b, Ir, Cr. iFrame "∗".
+    iFrame "%". iExists γ_hr, γ_ir. iFrame "∗#". iFrame "∗#".
   Qed.
 
   (** High-level lock specs *)
 
-  Lemma lockNode_spec_high γ_I γ_f γ_k γ_i γ_h r n :
+  Lemma lockNode_spec_high γ_I γ_f γ_k γ_gh r n :
     ⊢ inFP γ_f n
-      -∗ <<< ∀ C, CSS γ_I γ_f γ_k γ_i γ_h r C >>>
+      -∗ <<< ∀ C, CSS γ_I γ_f γ_k γ_gh r C >>>
            lockNode #n @ ⊤
-         <<< ∃ In Cn, CSS γ_I γ_f γ_k γ_i γ_h r C
-                      ∗ nodePred γ_f γ_h γ_k n In Cn,
+         <<< ∃ In Cn, CSS γ_I γ_f γ_k γ_gh r C
+                      ∗ nodePred γ_f γ_gh γ_k n In Cn,
              RET #() >>>.
   Proof.
     iIntros "#HFp". iIntros (Φ) "AU".
@@ -436,7 +507,7 @@ Section Link_Template.
     iApply (aacc_aupd_commit with "AU"); first done.
     iIntros (C) "Hcss".
     iPoseProof (CSS_unfold with "[$] [$]")
-      as (I) "(Hg & Hn & Hcss')".
+      as (hγ I) "(Hg & Hn & Hcss')".
     iSpecialize ("Hcss'" $! C).
     iDestruct "Hn" as (b In Cn) "(Hlock & Hns)".
     iAaccIntro with "Hlock".
@@ -453,22 +524,22 @@ Section Link_Template.
     iFrame "∗". iIntros "H". by iModIntro.
   Qed.
   
-  Lemma unlockNode_spec_high γ_I γ_f γ_k γ_i γ_h r n In Cn :
-    ⊢ nodePred γ_f γ_h γ_k n In Cn
-      -∗ <<< ∀ C, CSS γ_I γ_f γ_k γ_i γ_h r C >>>
+  Lemma unlockNode_spec_high γ_I γ_f γ_k γ_gh r n In Cn :
+    ⊢ nodePred γ_f γ_gh γ_k n In Cn
+      -∗ <<< ∀ C, CSS γ_I γ_f γ_k γ_gh r C >>>
            unlockNode #n @ ⊤
-         <<< CSS γ_I γ_f γ_k γ_i γ_h r C, RET #() >>>.
+         <<< CSS γ_I γ_f γ_k γ_gh r C, RET #() >>>.
   Proof.
     iIntros "Hnp". iIntros (Φ) "AU".
     awp_apply (unlockNode_spec n).
     iApply (aacc_aupd_commit with "AU"); first done.
     iIntros (C) "Hcss".
-    iDestruct "Hnp" as "(Hn & HnhIn & HkIn & #Hinfp & %)".
-    iPoseProof (CSS_unfold_node_wand with "[$] [$] [$] [$]")
-      as (I) "(Hn & HhIn & Hg & Hlock & Hns & Hcss')".
-    iAssert (nodePred γ_f γ_h γ_k n In Cn)%I 
+    iDestruct "Hnp" as (γ_hn γ_in) "(Hn & HnhIn & HkIn & #Hinfp & #Hgh)".
+    iPoseProof (CSS_unfold_node_wand with "[$] [$] [$] [$] [$]")
+      as (Hγ I) "(Hn & HhIn & Hg & Hlock & Hns & Hcss')".
+    iAssert (nodePred γ_f γ_gh γ_k n In Cn)%I 
         with "[Hn HkIn HhIn]" as "Hnp".
-    { iFrame "∗%#". }
+    { iFrame "∗%#". iExists γ_hn, γ_in. iFrame "∗#". }
     iCombine "Hlock" "Hnp" as "HPre".  
     iAaccIntro with "HPre".
     { iIntros "(Hlock & Hnp)". iModIntro.
@@ -484,18 +555,86 @@ Section Link_Template.
 
   (** Proofs of traverse and CSSOp *)
 
-  Lemma traverse_spec γ_I γ_f γ_k γ_i γ_h (r: Node) (k: K) (n: Node) :
-    ⊢ ⌜k ∈ KS⌝ -∗ inFP γ_f n -∗ inInr γ_i k n -∗
-        <<< ∀ C, CSS γ_I γ_f γ_k γ_i γ_h r C >>>
+  Theorem init_spec :
+   ⊢ {{{ True }}}
+        init #()
+     {{{ γ_I γ_f γ_k γ_gh (r: Node), RET #r; CSS γ_I γ_f γ_k γ_gh r ∅ }}}.
+  Proof.
+    iIntros (Φ). iModIntro.
+    iIntros "_ HΦ".
+    wp_lam. wp_apply createRoot_spec; try done.
+    iIntros (r Ir ks) "(node & Hl & HIr & Hks)".
+    iDestruct "HIr" as %HIr. iDestruct "Hks" as %Hks.
+    iApply fupd_wp.
+    iMod (own_alloc ( (● Ir) ⋅ (◯ Ir))) as (γ_I)"(HIr● & HIr◯)".
+    { apply auth_both_valid_discrete. split; try done.
+      unfold valid, cmra_valid. simpl. unfold ucmra_valid.
+      simpl. unfold flowint_valid. subst Ir.
+      split; try done. apply map_disjoint_dom. set_solver. }
+    iMod (own_alloc ((● prod (KS, ∅)) ⋅ (◯ (prod (KS, ∅))))) 
+          as (γ_k)"(Hks● & Hks◯)".
+    { apply auth_both_valid_discrete. split; try done. }
+    iMod (own_alloc (● (domm Ir) ⋅ ◯ (domm Ir))) 
+          as (γ_f)"(Hf & #Hf')". 
+    { apply auth_both_valid_discrete. try done. }
+    iMod (own_alloc (to_frac_agree (1) Ir)) 
+          as (γ_hr)"HhIn". { try done. }
+    iEval (rewrite <-Qp_half_half) in "HhIn".      
+    iEval (rewrite (frac_agree_op (1/2) (1/2) _)) in "HhIn". 
+    iDestruct "HhIn" as "(HhIn & HhIn')".
+    iMod (own_alloc (● inset K Ir r)) 
+          as (γ_ir)"HInr". { apply auth_auth_valid. try done. }
+    iMod (own_alloc (● {[r := to_agree (γ_hr, γ_ir)]} 
+                      ⋅ ◯ {[r := to_agree (γ_hr, γ_ir)]}  ) ) 
+          as (γ_gh)"(Hgh● & #Hgh◯)". 
+    { apply auth_both_valid_discrete. split; try done.
+      apply singleton_valid. try done. }
+    iModIntro. wp_pures.
+    iModIntro. iApply ("HΦ" $! γ_I γ_f γ_k γ_gh r).
+    iExists {[r := to_agree (γ_hr, γ_ir)]}, Ir. iFrame. iSplitR.
+    - iPureIntro. repeat split; try done.
+      unfold valid, cmra_valid, flowint_valid.
+      subst Ir; split; try done.
+      apply map_disjoint_dom; set_solver.
+      subst Ir. unfold domm, dom, flowint_dom. simpl.
+      rewrite dom_singleton. set_solver.
+      unfold closed, outset, dom_ms, out, out_map.
+      subst Ir; simpl. try done.
+      unfold inset, dom_ms, inf.
+      subst Ir; simpl. rewrite lookup_singleton; simpl.
+      intros k Hk; rewrite Hks; try done.
+    - assert (domm Ir = {[r]}) as Domm_Ir.
+      { subst Ir; unfold domm, dom, flowint_dom, inf_map; simpl.
+        apply leibniz_equiv. by rewrite dom_singleton. }
+      rewrite Domm_Ir. rewrite big_opS_singleton.
+      iExists false, Ir, ∅. iFrame "∗%".
+      assert (keyset K Ir r = KS) as Hkeyset.
+      { unfold keyset. unfold dom_ms, inf, out; subst Ir; simpl.
+        rewrite nzmap_lookup_empty. rewrite lookup_singleton.
+        unfold ccmunit at 2. unfold ccm_unit. simpl.
+        unfold nzmap_dom. simpl.
+        assert (dom (gset K) (∅: gmap K nat) = ∅) as H'.
+        { apply leibniz_equiv. by rewrite dom_empty. }
+        rewrite H' Hks. set_solver. }
+      iSplitL "HhIn Hks◯". iExists γ_hr, γ_ir.   
+      rewrite Hkeyset. iFrame "∗#". iExists {[r]}. iFrame "#".
+      by iPureIntro; clear; set_solver.
+      iExists γ_hr, γ_ir. iFrame "∗#".  
+  Qed.
+
+  Lemma traverse_spec γ_I γ_f γ_k γ_gh γ_hn γ_in (r: Node) (k: K) (n: Node) :
+    ⊢ ⌜k ∈ KS⌝ -∗ inFP γ_f n -∗ 
+        own γ_gh (◯ {[n := to_agree (γ_hn, γ_in)]}) -∗ inInr γ_in k -∗
+        <<< ∀ C, CSS γ_I γ_f γ_k γ_gh r C >>>
             traverse #n #k @ ⊤
         <<< ∃ (n': Node) (In': multiset_flowint_ur K) (Cn': gset K),
-            CSS γ_I γ_f γ_k γ_i γ_h r C
-            ∗ nodePred γ_f γ_h γ_k n' In' Cn'
+            CSS γ_I γ_f γ_k γ_gh r C
+            ∗ nodePred γ_f γ_gh γ_k n' In' Cn'
             ∗ ⌜in_inset K k In' n'⌝ ∗ ⌜¬in_outsets K k In'⌝,
             RET #n'
         >>>.
   Proof.
-    iLöb as "IH" forall (n). iIntros "% #Hinfp #Hininr".
+    iLöb as "IH" forall (n γ_hn γ_in). iIntros "% #Hinfp #Hgh #Hininr".
     iIntros (Φ) "AU". wp_lam. wp_let. wp_bind(lockNode _)%E.
     awp_apply lockNode_spec_high; first done.
     (* Open AU to get lockNode pre *)
@@ -505,12 +644,14 @@ Section Link_Template.
     { iIntros "H". iModIntro. iFrame. iIntros. iModIntro. iFrame. }
     iIntros (In Cn) "(Hcss & Hnp)". iModIntro.
     (* Before closing AU, use CSS to get findNext pre *)
-    iPoseProof (inInr_impl_inset with "[$] [$] [$]")
+    iPoseProof (inInr_impl_inset with "[$] [$] [$] [$]")
       as "%".
     (* Close AU and move on *)
     iFrame. iIntros "AU". iModIntro.
     wp_pures.
-    iDestruct "Hnp" as "(Hn & HnhIn & HkIn & _ & %)".
+    iDestruct "Hnp" as (γ_hn' γ_in')"(Hn & HnhIn & HkIn & _ & #Hgh')".
+    iPoseProof (ghost_heap_sync _ _ _ _ with "[$Hgh] [$Hgh']") as "(% & %)". 
+    subst γ_hn' γ_in'.    
     wp_bind (findNext _ _)%E. wp_apply ((findNext_spec n k In Cn) with "[$Hn]").
     { iPureIntro; split; done. }
     iIntros (b n') "(Hn & Hout)". destruct b.
@@ -518,12 +659,14 @@ Section Link_Template.
       wp_pures. wp_bind (unlockNode _).
       iDestruct "Hout" as %Hout.
       (* Fold nodePred again *)
-      iAssert (nodePred γ_f γ_h γ_k n In Cn)%I
-        with "[$Hn $HnhIn $HkIn $Hinfp]" as "Hnp"; first by iPureIntro.
+      iAssert (nodePred γ_f γ_gh γ_k n In Cn)%I
+        with "[Hn HnhIn HkIn Hinfp]" as "Hnp".
+      { iExists γ_hn, γ_in. iFrame "∗#". }
       (* Get traverse's pre before giving up (node n) when calling unlock *)
       iApply fupd_wp. clear C. iMod "AU" as (C) "[Hcss [Hclose _]]".
+      iClear "Hgh'".
       iMod (ghost_update_step with "[$] [$] [% //] [% //]")
-        as "(Hcss & Hnp & #Hinfp' & #Hininr')".
+        as (γ_hn' γ_in')"(Hcss & Hnp & Hgh' & Hinfp' & Hininr')".
       (* Close AU after getting traverse's pre *)
       iMod ("Hclose" with "Hcss") as "AU". clear C. iModIntro.
       awp_apply (unlockNode_spec_high with "Hnp").
@@ -536,32 +679,33 @@ Section Link_Template.
       (* Close up AU again *)
       iFrame. iIntros "AU". iModIntro. 
       wp_pures. iSpecialize ("IH" $! n').
-      iApply ("IH" with "[% //] [$] [$]"). done.
+      iApply ("IH" with "[% //] [$] [$] [$]"). done.
     - (* Case: findNext returns None *)
       (* Open AU and commit *)
       iApply fupd_wp. clear C. iMod "AU" as (C) "[Hcss [_ Hclose]]".
       iSpecialize ("Hclose" $! n In Cn).
-      iAssert (nodePred γ_f γ_h γ_k n In Cn)%I
-        with "[$Hn $HnhIn $HkIn $Hinfp]" as "Hnp"; first by iPureIntro.
+      iAssert (nodePred γ_f γ_gh γ_k n In Cn)%I
+        with "[Hn HnhIn HkIn Hinfp]" as "Hnp".
+      { iExists γ_hn, γ_in. iFrame "∗#". }
       iMod ("Hclose" with "[$Hcss $Hnp $Hout]") as "HΦ"; first by iPureIntro.
       iModIntro. wp_pures. done.
   Qed.
 
   (** Verification of abstract specification of the search structure operation. *)
     
-  Theorem CSSOp_spec (γ_I γ_f γ_k: gname) γ_i γ_h r (k: K) (dop: dOp):
-    ⌜k ∈ KS⌝ -∗ <<< ∀ C, CSS γ_I γ_f γ_k γ_i γ_h r C >>>
+  Theorem CSSOp_spec γ_I γ_f γ_k γ_gh r (k: K) (dop: dOp):
+    ⌜k ∈ KS⌝ -∗ <<< ∀ C, CSS γ_I γ_f γ_k γ_gh r C >>>
       CSSOp dop r #k @ ⊤
-    <<< ∃ C' (res: bool), CSS γ_I γ_f γ_k γ_i γ_h r C'
+    <<< ∃ C' (res: bool), CSS γ_I γ_f γ_k γ_gh r C'
         ∗ ⌜Ψ dop k C C' res⌝, RET #res >>>.
   Proof.
     iIntros "%" (Φ) "AU". iLöb as "IH". wp_lam.
     (* Open AU for traverse's pre *)
     iApply fupd_wp. iMod "AU" as (?) "[Hcss [Hclose _]]".
-    iMod (ghost_update_root with "[$] [% //]") as "(Hcss & ? & ?)".
+    iMod (ghost_update_root with "[$] [% //]") as (γ_hr γ_ir) "(Hcss & #Hghr & #inFP_r & #inInr_k)".
     iMod ("Hclose" with "[$] ") as "AU".
     iModIntro. wp_bind (traverse _ _)%E.
-    awp_apply (traverse_spec with "[% //] [$] [$]").
+    awp_apply (traverse_spec with "[% //] [$] [$]"); try done.
     (* Open AU for traverse's atomic pre *)
     iApply (aacc_aupd_abort with "AU"); first done.
     iIntros (?) "Hcss".
@@ -572,7 +716,7 @@ Section Link_Template.
     iModIntro. iFrame. iIntros "AU". iModIntro.
     (* Execute decisiveOp *)
     wp_pures. wp_bind (decisiveOp _ _ _)%E.
-    iDestruct "Hnp" as "(Hn & HnhIn & HkIn & #Hinfp & %)".
+    iDestruct "Hnp" as (γ_hn γ_in)"(Hn & HnhIn & HkIn & #Hinfp & #Hgh)".
     wp_apply (decisiveOp_spec with "[$Hn]"); first by iPureIntro.
     iIntros (b res Cn'). iIntros "(Hn & Hb)". destruct b.
     - (* Case: decisiveOp succeeds *)
@@ -590,8 +734,8 @@ Section Link_Template.
       iApply (aacc_aupd_commit with "AU"); first done.
       iIntros (C) "Hcss".
       (* Now unfold CSS to execute unlockNode *)
-      iPoseProof (CSS_unfold_node_wand with "[$] [$] [$] [$]")
-        as (I) "(Hn & HhIn & Hg & Hlock & Hns & Hcss')".
+      iPoseProof (CSS_unfold_node_wand with "[$] [$] [$] [$] [$]")
+        as (Hγ I) "(Hn & HhIn & Hg & Hlock & Hns & Hcss')".
       iDestruct "Hlock" as "(Hlock & _)".
       iAaccIntro with "Hlock".
       { iIntros "Hlock". iModIntro.
@@ -616,12 +760,14 @@ Section Link_Template.
       (* Close everything up, return *)
       iModIntro. iExists C', res. iSpecialize ("Hcss'" $! C').
       iPoseProof ("Hcss'" with "[-]") as "Hcss".
-      { iFrame "∗". iExists false, In, Cn'. iFrame "∗#%". }
+      { iFrame "∗". iExists false, In, Cn'. iFrame "∗#%".
+        iExists γ_hn, γ_in. iFrame "∗#". }
       iFrame "Hcss HΨC". iIntros "H". iModIntro. wp_pures. done.
     - (* Case: decisiveOp fails *)
       wp_pures. iDestruct "Hb" as "%". subst Cn'.
-      iAssert (nodePred γ_f γ_h γ_k n In Cn)%I
-        with "[$Hn $HnhIn $HkIn $Hinfp //]" as "Hnp". 
+      iAssert (nodePred γ_f γ_gh γ_k n In Cn)%I
+        with "[Hn HnhIn HkIn Hinfp]" as "Hnp".
+      { iExists γ_hn, γ_in. iFrame "∗#". }
       awp_apply (unlockNode_spec_high with "Hnp").
       (* Open AU for unlockNode's pre *)
       iApply (aacc_aupd_abort with "AU"); first done. iIntros (C) "Hcss".
